\documentclass{article}
\usepackage{amsmath,amssymb}
\usepackage{hyperref}
\title{CSC165 Fall 2014, Assignment 2}
\author{Anish Krishna, Connor Peet, George Wu}
\renewcommand{\today}{~}
\hypersetup{pdfpagemode=Fullscreen,
  colorlinks=true,
  linkfileprefix={}}
\newcommand{\floor}[1]{\lfloor #1\rfloor}
\begin{document}
\maketitle
\noindent
The aim of this assignment is for you to practice devising and
presenting proofs.  You may work in groups of no more than three
students, and you should produce a single solution in a PDF file named
\texttt{a2.pdf}, submitted to
\href{https://markus.cdf.toronto.edu/csc165-2014-09}{MarkUs}.

You will receive 20\% of the marks for any question you either leave
blank, or write ``I cannot answer this.''  You will receive 0 for any
false claim you ``prove,'' or any true claim you ``disprove.''

\begin{enumerate}
\item Proving the statement 1.1 true.  %1.1
    \begin{description}
    \item Assume $x \in \mathbb{R}$ \# generic
        \begin{description}
        \item Assume $y \in \mathbb{R}$ \# generic
            \begin{description}
            \item Assume $x > y$ \# Antecedent
                \begin{description}
                \item Then $\forall z \in \mathbb{Z}, z \leq x \implies z \leq \floor{x}$ and $\forall z \in \mathbb{Z}, z \leq y \implies z \leq \floor{y}$\# Definition of floor
                \item Then $\forall z \in \mathbb{Z}, z \leq y \implies (z \leq \floor{x} \land z \leq \floor{y})$ \# $x < y$, so by the antecedent $z \leq y \implies z \leq x$
                \item Let there be $d = (x - y) / 1$ \# Treat as integer division.
                \item Then $d \in \mathbb{N}_0$ \# d must be $\geq$ zero because $x > y$, and closed under division.
                \item Then $\forall z \in \mathbb{Z}, z \leq y \implies (z + d \leq \floor{x} \land z \leq \floor{y})$ \# Make the $x$ part of the and statement equivalent to its definition.
                \item Then $\floor{x} \leq \floor{y}$ \# $z < z + d$
                \end{description}
            \item Conclude $x > y \implies \floor{x} \geq \floor{y}$
            \end{description}
        \item Conclude $\forall y \in \mathbb{R}, x < y \implies \floor{x} \geq \floor{y}$
        \end{description}
    \item Conclude $\forall x \in \mathbb{R}, \forall y \in \mathbb{R}, x < y \implies \floor{x} \geq \floor{y}$
    \end{description}

\item Proving the statement 1.2 true.   %1.2
    \begin{description}
    \item Assume $x \in \mathbb{R}, e \in \mathbb{R}^+$ \# generic
        \begin{description}
        \item Let $d = e + 2$
        \item Then $d \in \mathbb{R}^+$ \# $\mathbb{R}^+$ closed by addition
        \item Assume $w \in \mathbb{R}$ \# generic
            \begin{description}
            \item Assume $\mid x - w \mid < d$ is true \# antecedent
                \begin{description}
                \item Then $w - 1 < \floor{w} \leq w$ and $x - 1 < \floor{x} \leq x$ \# By definition of floor, $\forall z \in \mathbb{Z}, z \leq x \implies z \leq \floor{x}$ and $\floor{x} \leq x$
                \item Then $\mid\floor{x} - x\mid = 1$ and $\mid\floor{w} - w \mid = 1$ \# therefore the floor of a value will therefore always be within $\pm 1$ of the value
                \item Then $\mid (\floor{x} \pm 1) - (\floor{w} \pm 1) \mid < e + 2$ \# Using the antecedent, sub in for $x$ and $w$.
                \item Then $\mid \floor{x} - \floor{w} \pm 2 \mid < e + 2$ \# Associative property of addition
                \item Then $\mid \floor{x} - \floor{w} \mid + 2 < e + 2$ \# move the $\pm$s out of the absolute value; they become simply positive two at maximum and zero at minimum, so the inequality holds.
                \item Then $\mid \floor{x} - \floor{w} \mid < e$ \# Subtract 2 from both sides.
                \end{description}

            \item Then $\mid x - w \mid < d \implies \mid \floor{x} - \floor{y} \mid < e$
            \end{description}
        \item Then $\exists d \in \mathbb{R}^+, \forall w \in \mathbb{R}, \mid x - w \mid < d \implies \mid \floor{x} - \floor{y} \mid < e$
        \end{description}
    \item Then $\forall x \in \mathbb{R}, \forall e \in \mathbb{R}^2, \exists d \in \mathbb{R}^+, \forall w \in \mathbb{R}, \mid x - w \mid < d \implies \mid \floor{x} - \floor{y} \mid < e$
    \end{description}

\item Proving the statement 1.3 true. %1.3
    \begin{description}
    \item Let $x = 0.5$ \# 0.5 is a positive real number
    \item Then $x \in \mathbb{R}$
    \item Assume $e \in \mathbb{R}^+$ \# Generic
        \begin{description}
        \item Let $d = 0.1$
        \item Then $d \in \mathbb{R}^+$ \# 0.1 is a positive real number
        \item Assume $w \in \mathbb{R}$ and that $\mid x - w \mid < d$
            \begin{description}
            \item Then $0.4 < w < 0.6$ \# Difference between x (0.5) and w is less than 0.1.
            \item Then $\floor{w} = \floor{x} = 0$ \# From definition of floor
            \item Then $\mid \floor{x} - \floor{w} \mid = 0$ \# Zero minus zero is simply zero.
            \item Then $\mid \floor{x} - \floor{w} \mid < e$ \# Zero is less than all positive real numbers, by definition of positive.
            \end{description}
        \item Then $\forall w\in\mathbb{R}, |x-w|< d \implies |\lfloor x\rfloor - \lfloor w\rfloor| < e$
        \end{description}
    \item Then $\exists x\in\mathbb{R}, \forall e \in\mathbb{R}^+, \exists d \in\mathbb{R}^+, \forall w\in\mathbb{R}, |x-w|< d \implies |\lfloor x\rfloor - \lfloor w\rfloor| < e$
    \end{description}

\item Proving 1.4 False. %1.4
		\begin{description}
		\item The negation of claim 1.4 would be:
		\item $\forall x \in \mathbb{R} \floor{x+1} = \floor{x} + 1$
				\begin{description}
				\item Assume $x \in \mathbb{R}$ \# Generic
						\begin{description}
						\item $\exists Z_{0}$ such that $Z_0 \leq x+1 \wedge \forall Z_0 \in \mathbb{Z} Z_0 \leq x+1 \Rightarrow Z_0 \leq \floor{x+1}$ \# Definition of floor.
						\item $\exists Z_1$ such that $Z_1 \leq x \wedge \forall Z_1 \in \mathbb{Z}, Z_1 \leq x \Rightarrow Z_1 \leq \floor{x}$ \# Definition of floor.
						\item Then $Z_0 = \floor{x+1}$ and $Z_1 = \floor{x}$
						\item Then, $Z_{0} - 1 \leq x$ \# $Z_0$ is the largest integer less than or equal to x+1. Then, $Z_0 - 1$ is the largest integer less than x, since subtracting one from both sides of the inequality $Z_0 \leq x +1$ will give the largest integer less than x.
						\item Then $Z_1 \leq x$ \# By definition of floor, $Z_1$ is also the largest integer less than or equal to x.
						\item Then $Z_0 -1 = Z_1$ \# The largest integer less than or equal to x must be the same values.
						\item Then $Z_0 = Z_1 + 1$ \# Add one to both sides.
						\end{description}
				\item Then, $\floor{x+1} = \floor{x}+1$\# Substitute in the values of $Z_0$ and $Z_1$
				\end{description}
		\item Then $\forall x \in \mathbb {R}$, $\floor{x+1} = \floor{x} + 1$
		\end{description}

\item Proving 2.1 is true, and proving the converse of 2.1 is false.
		\begin {description}
				\item Let n be any natural number. \# Domain assumption.
				\begin{description}
						\item Assume, $\exists k \in \mathbb{N}, n = 5k_0 + 2$ \# Antecedent
							\begin{description}
							\item Let $j = 5k^2 + 4k$ \#
							\item Then $j \in \mathbb{N}$, since natural numbers closed under addition, multiplication.
							\item Then $n^2 = (5k + 2)(5k + 2) = 25 k^2 + 20k + 4 = 5(5k^2 + 4k) + 4$ \# Substituting in antecedent for $n^2$
							\item Then $n^2 = 5j + 4$ \# Substituting $j$ into the equation.
							\item Then $\exists j \in \mathbb{N}, n^2 = 5j + 4$
							\end{description}
						\item Then $(\exists k \in \mathbb{N}, n = 5k + 2) \implies (\exists j \in \mathbb{N}, n^2 = 5j + 4)$ such that $n^2 = 5j+4$
				\end {description}
				\item Then $\forall n \in \mathbb{N}$, $\exists k \in \mathbb{N}, n = 5k+2 \Rightarrow \exists j \in \mathbb{N}, n^2 = 5j+4$ \#Thus, proving the negation of the statement disproves the statement
		\end {description}

Proving the converse of 2.1 is false:\\
The converse of 2.1 would be:\\
$\forall n \in \mathbb{N}$, ($\exists j \in \mathbb{N}, n^2 = 5j+4) \Rightarrow (\exists k \in \mathbb{N}, n = 5k+2$)\\
The negation of the converse of 2.1 would be:\\
$\exists n \in \mathbb{N}$, ($\exists j \in \mathbb{N}, n^2 = 5j+4) \wedge (\forall k \in \mathbb{N}, n \neq 5k+2$)
		\begin {description}
				\item Choose $n = 3$ \# $n \in \mathbb{N}$
				\item Let $j \in \mathbb{N}, j = 1$, then $\exists j \in \mathbb{N}, n^2 = 5j+4$ is true.
				\item Then the latter statement is $\forall k \in \mathbb{N}, 3 \neq 5k + 2$
				\item Then it may be simplified as $\forall k \in \mathbb{N}, 1 \neq 5k$
				\item 5 does not divide 1, therefore the latter statement is false.
				\item Then, $\exists n \in \mathbb{N}$, ($\exists j \in \mathbb{N}, n^2 = 5j+4) \wedge (\forall k \in \mathbb{N}, n \neq 5k+2$) \# We've proved the negation of the converse, so we disproved the converse.
\end{description}

\item Proving claim 2.2 is true, and disproving its converse.
		\begin{description}
				\item Assume $m, n \in \mathbb{R}$ \# generic
						\begin{description}
						\item Let $k_0$, $j_0$ be a natural numbers
						\item Assume $m = 7k_0 + 3$ and $n = 7j_0 + 4$ \# Antecedent
								\begin{description}
								\item Then, evaluating $mn$, we get $mn = (7k_0 + 3)(7j_0 +4)$
								\item $mn = 49k_0j_0 + 28k_0 + 21j_0 + 12$ \# Expand the product
								\item $mn = 49k_0j_0 + 28k_0 + 21j_0 + 7 + 5$ \# Change 12 into 7+5
								\item $mn = 7(7k_0j_0 + 6k_0 + 3j_0 + 1) +5$ \# Factor out 7 from the first 4 terms.
								\end {description}

						\item Let $i_0 = 7k_0j_0 + 6k_0 + 3j_0 + 1$
						\item Then $i_0 \in \mathbb{N}$ \# Natural numbers are closed under addition and multiplication.
						\item Then $mn = 7i_0 + 5$ \# Substitute in i
						\end{description}
				\item Then, $\forall m,n \in \mathbb{N}$, ($\exists k \in \mathbb{N}, m = 7k + 3$) $\wedge$ ($\exists j \in \mathbb{N}, n = 7j + 4$) $\Rightarrow$ ($\exists i \in \mathbb{N}, mn = 7i + 5$)
		\end{description}

Proving the converse of 2.2 is false. We will continue by finding the converse, and then proving the negation of its contrapositive.\\

The converse of 2.2 is $\forall m,n$ ($\exists i \in \mathbb{N}, mn = 7i + 5$) $\Rightarrow$ ($\exists k \in \mathbb{N}, m = 7k + 3$) $\wedge$ ($\exists j \in \mathbb{N}, n = 7j + 4$)\\
Its contrapositive is $\forall m,n$ ($\forall k \in \mathbb{N}, m \neq 7k+3$) $\vee$ ($\forall j \in \mathbb{N}, n \neq 7j + 4$) $\Rightarrow$ $\forall i \in \mathbb{N} mn \neq 7i + 5$\\
The negation is $\exists m,n$ ($\forall k \in \mathbb{N}, m \neq 7k + 3$) $\vee$ ($\forall j \in \mathbb{N}, n \neq 7j + 4$) $\Rightarrow$ ($\exists i \in \mathbb{N}, mn = 7i + 5)$.\\
		\begin{description}
			\item Let $m \in \mathbb{N}, m = 10$
			\item Then $\forall k \in \mathbb{N}, m \neq 7k + 3$ is false. \# There exists $k$ with value of 1 which causes it to evaluate false.
			\item Let $n \in \mathbb{N}, n = 11$
			\item Then $\forall j \in \mathbb{N}, n \neq 7j + 4$ is false. \# There exists $j$ with value of 1 which causes it to evaluate false.
			\item Then the antecedent is always false and, therefore, the implication is true.
		
		\item Then, $\exists m,n$ ($\forall k \in \mathbb{N}, m \neq 7k + 3$) $\vee$ ($\forall j in \mathbb{N}, n \neq 7j + 4$) $\Rightarrow$ $\exists i \in \mathbb{N} mn = 7i + 5$ \# Assumed antecendent, got consequent.
		\end{description}

\end{enumerate}

\end{document}
