\documentclass{article}
\usepackage{amsmath,amssymb}
\usepackage{hyperref}
\title{CSC165 Fall 2014, Assignment 3}
\author{Anish Krishna, Connor Peet, George Wu}
\renewcommand{\today}{~}
\hypersetup{pdfpagemode=Fullscreen,
  colorlinks=true,
  linkfileprefix={}}
\newcommand{\floor}[1]{\lfloor #1\rfloor}
\begin{document}
\maketitle


\begin{enumerate}
\item Proving the statement 1 true.
    \begin{description}
    \item Assume $e \in \mathbb{R}^+$ \# generic
    		\begin{description}
    		\item Let $d = e$
    		\item Then $d \in \mathbb{R}^+$ \# e is a positive, real number.
    		\item Assume $x, y \in \mathbb{R}^+$ and that $|x - y| > d$ \# Generic, antecedent assumption
    			\begin{description}
    			\item Then $x + y = |x + y|$ \# $\mathbb{R}^+$ closed by addition, the absolute value of a positive number is that number.
    			\item Also $x + y > |x - y|$ \# The sum of two positive real numbers will always be greater than their difference.
    			\item Then $|x + y| > d$ \# Sub in, by antecedent
    			\item Then $|x + y| > e$
    			\end{description}
    		\end{description}
    \item Then $\forall e \in \mathbb{R}^+, \exists d \in \mathbb{R}^+, \forall x, y \in \mathbb{R}^+, |x - y| > d \implies |x + y| > e$.
    \end{description}
\item Proving statement 2 true, where $f(n) = 6n^3 - 4n^2 + 3n + 2$ and $g(n) = 5n^3 - n^2 + n + 1$
	\begin{description}
	\item Let $c = 1$
	\item Then $c \in \mathbb{R}^+$ \# 1 is a positive real number.
	\item Let $b = 3$
	\item Then $c \in \mathbb{N}$ \# 3 is a natural number.
	\item Assume $n \in \mathbb{N}$
		\begin{description}
		\item Then $f(n) = 6n^3 - 4n^2 + 3n + 2$
		\item Then $f(n) \geq 6n^3 - 4n^2 + n + 1$ \# Subtract $2n + 1$, which is greater than zero because $n \in \mathbb{R}^+$
		\item Then $f(n) \geq 5n^3 - n^2 + n + 1$ \# Subtract $n^3 - 3n^2$, which is greater than or equal to zero because $n \geq 3$
		\item Then $f(n) \geq g(n)$ \# Substitue in $g(n)$
		\item Then $f(n) \geq cg(n)$ \# $c = 1$, identity property of multiplication
		\end{description}
	\item Then $\exists c \in \mathbb{R}^+, \exists B \in \mathbb{N}, \forall n \in n, n \geq B \implies f(n) \geq cg(n)$
	\item Then $6n^3 - 4n^2 + 3n + 2 \in \Omega(5n^3 - n^2 + n + 1)$
	\end{description}
	
\item Proving number 3 is false.
	\begin{description}
		\item Using l'Hopital's rule, we know that:	
		\begin{equation*}
		\lim_{x\to\infty}\frac{15n^2}{3 \times 2^n}=0
		\end{equation*}
		\item Negation of the given statement is the following: $\forall B \in \mathbb{N}, \forall c \in \mathbb{R}, \exists n \in \mathbb{N}, n\geq B \wedge 15n^2 < c\times 3 \times 2^n$
		\item Assume $B \in \mathbb{N}, c \in \mathbb{R}^+$.
		\begin{description}
			\item Then $\forall e \in \mathbb{R}^+, \exists M \in \mathbb{N}, \forall n \in \mathbb{N}, n \geq M \Rightarrow L - e < \frac{15n^2}{3\times n^2}< L + e$ \# Definition of limit
			\item Then $\forall e \in \mathbb{R}^+, \exists M \in \mathbb{N}, \forall n \in \mathbb{N}, n \geq M \Rightarrow -e < \frac{15n^2}{3\times n^2}< e$ \# L = 0, by l'Hopital's rule
			\item Then, $\exists M \in \mathbb{N}, \forall n \in \mathbb{N}, n \geq M \Rightarrow \frac{15n^2}{3\times n^2} < c$ \# We let e = c.
			\item Let $M$ be such that $\forall n \in \mathbb{N}, n \geq M \Rightarrow \frac{15n^2}{3\times n^2} < c$ and choose $n = \max(M,B)$
			\item Then $n \in \mathbb{N}$
			\item Then $n \geq B$ \# By definition of maximum.
			\item Then $15n^2 < c \times 3 \times 2^n$\#Multiplying $3\times 2^n$ over the inequality. We know this is true because $2^n$ is positive, so this will not change the inequality.
			\item Then $n \geq B$ and $15n^2 < c\times 3\times 2^n$.
		\end{description}
		\item Then $\forall B \in \mathbb{N}, \forall c \in \mathbb{R}, \exists n \in \mathbb{N}, n\geq B \wedge 15n^2 < c\times 3 \times 2^n$
	\end{description}
	
\item Proving number 4 true.
\begin{description}
	\item We know that:
	\begin{equation*}
		\lim_{x\to\infty}\frac{2^n}{3^n}=\lim_{x\to\infty} \left(\frac{2}{3}\right)^n = 0
	\end{equation*}
	\item Pick $c = 1$, $B = 0$
	\item Assume $n$ to be any natural number and $n \geq B$
	\begin{description}
		\item Then $\exists M \in \mathbb{N}, \forall n_1 \in \mathbb{N}, n_1 \geq M \Rightarrow -c< \frac{2^{n_1}}{3^{n_1}} < c$ \# We know that the limit exists, so we simply set e = c.
		\item Choose $M = B$.
		\item Then we know that $\forall n_1 \in \mathbb{N}, n_1 \geq B \Rightarrow \frac{2^{n_1}}{3^{n_1}} < 1$ \# Since c = 1.
		\item Then $n_1 \in \mathbb{N}$ and $n_1 \geq M = B$
		\item Then $n_1$ describes the same set of numbers as $n$
		\item Then $\frac{2^{n_1}}{3^{n_1}} = \frac{2^n}{3^n} < 1$ \# Setting c = 1.
		\item Then $2^n < 3^n$ \# since $n \geq M$, so we know that $3^n$ is positive.
		\item Then $n \geq B \Rightarrow 2^n < 3^n$ \# Assumed antecedent and got conclusion.
	\end{description}
	\item Then $\exists B \in \mathbb{N}, \exists c \in \mathbb{R}^+, \forall n \in \mathbb{N}, n \geq B \Rightarrow 2^n \leq 3^n$
\end {description}
\item Proving number 5 to be true.
\begin{description}
	\item Defininition of $\mathcal{O}(g):\\ \exists c \in \mathbb{R}^+, \exists B \in \mathbb{N}, \forall n \in n, n \geq B \implies f(n) \leq cg(n)$
	\item Defininition of $\Omega(g):\\ \exists c \in \mathbb{R}^+, \exists B \in \mathbb{N}, \forall n \in n, n \geq B \implies f(n) \geq cg(n)$
	\item Assume f,g $\in \mathcal{F}$
	\item Let $c = \mathbb{R}^+$
	\item Let B $\in \mathbb{N}$
	\item Assume n $\in \mathbb {N}$
	\begin{description}
		\item Case 1:
			\begin{description}
			\item Assume f(n) $\leq$ cg(n)
			\item Then Case 1 satisfies definition of $\mathcal{O}(g)$
			\end{description}
		\item Case 2:
			\begin{description}
			\item Assume f(n) $\geq$ cg(n)
			\item Then $\lnot(f(n) \leq cg(n)) = f(n) > cg(n)$ 
			\item Then Case 2 satisfies defintition of $\Omega(g)$  \# $ f(n) > cg(n) = f(n) \geq cg(n)$
			\end{description}
		\item Then Case 1 and Case 2 covers all possible cases
	\end{description}
	\item Then $f\in\mathcal{O}(g) \vee f\in\Omega(g)$
	\item Then $\forall f, g\in\mathcal{F}, f\in\mathcal{O}(g) \vee f\in\Omega(g)$
\end {description}

\item Proving that the function \verb+meaning_of_life+ below is not computable:   %6
Using proof by contradiction to prove non-computability. 
\begin{description}
	\item Assume  \verb+meaning_of_life+ is computable 
	\begin{description}
		\item Then 
		\begin{verbatim}
		def meaning_of_life(f, I):
		 	"""Return True if f(I) returns 42, False otherwise."""
			# Implementation omitted

		def halt(f, i) :
		   def P(x) :
		      f(i)
		      if True:
		         return 42
		   return meaning_of_life(P, x)
		\end{verbatim}
		\item Then the if statement block under halt function executes iff f(i) halts.
		\item Then halt(f, i) returns True if f(i) halts, else it will return False. 
		\item Contradiction. Halt functions are non-computable  \# General specification of halt functionality
	\end{description}
	\item Then  \verb+meaning_of_life+ is non-computable 


\end {description}
\end{enumerate}

\end{document}

% LocalWords:  brachial
